prove seq branch of ceval'_derive

ASTLc_woc.v
@@ -1,5 +1,6 @@
 Require Import Coq.Lists.List.
 Require Import AST_woc.
+Require Import Omega.
 
 Require Import Coq.Relations.Relation_Operators.
 Require Import Coq.Relations.Relation_Definitions.
@@ -205,27 +206,100 @@ Inductive ceval' : func_context -> com -> label -> label -> state -> state -> Pr
   | E'_Reentryr2 : forall fc st,
       ceval' fc CReentry LHere LPure st st
 .
+
+Lemma ceval'_valid_label : 
+  forall fc c l1 l2 st1 st2,
+  ceval' fc c l1 l2 st1 st2 ->
+  valid_label l1 /\ valid_label l2.
+Proof.
+  intros.
+  inversion H; subst;
+  try (split; left; apply IP_Pure);
+  try pose proof com_to_label_pure_is_pure c1 as Hpc1;
+  try pose proof com_to_label_pure_is_pure c2 as Hpc2;
+  try pose proof com_to_label_pure_is_pure c0 as Hpc0.
+  - destruct H0, H3.
+    split; left; apply IP_Seq; assumption.
+    split. left; apply IP_Seq; assumption.
+           right; apply SP_Seq2; assumption.
+    split. right; apply SP_Seq1; assumption.
+           left; apply IP_Seq; assumption.
+    split. right; apply SP_Seq1; assumption.
+           right; apply SP_Seq2; assumption.
+  - split.
+    destruct H0.
+    left; apply IP_Seq; assumption.
+    right; apply SP_Seq1; assumption.
+    right; apply SP_Seq1; assumption.
+  - split.
+    right; apply SP_Seq2; assumption.
+    destruct H1.
+    left; apply IP_Seq; assumption.
+    right; apply SP_Seq2; assumption.
+  - split.
+    left; apply IP_If; assumption.
+    destruct H1.
+    left; apply IP_If; assumption.
+    right; apply SP_If1; assumption.
+  - split.
+    left; apply IP_If; assumption.
+    destruct H1.
+    left; apply IP_If; assumption.
+    right; apply SP_If2; assumption.
+  - split.
+    right; apply SP_If1; assumption.
+    destruct H1.
+    left; apply IP_If; assumption.
+    right; apply SP_If1; assumption.
+  - split.
+    right; apply SP_If2; assumption.
+    destruct H1.
+    left; apply IP_If; assumption.
+    right; apply SP_If2; assumption.
+  - split;
+    left; apply IP_While; assumption.
+  - split.
+    left; apply IP_While; assumption.
+    right; apply SP_While; assumption.
+  - split.
+    left; assumption.
+    assumption.
+  - split; right; apply SP_While; assumption.
+  - split.
+    right; assumption.
+    assumption.
+  - split.
+    left; apply IP_Pure.
+    right; apply SP_Here.
+  - split.
+    right; apply SP_Here.
+    left; apply IP_Pure.
+Qed.
 (** [] *)
 
 
 (** Bridging basic ceval' to multi_ceval' *)
-Definition restk : Type := list (com * label * state).
+Definition restk : Type := list (com * (option label) * state).
 
 Inductive middle_ceval' : func_context -> public_funcs -> restk -> restk -> Prop :=
-  | ME_r : forall fc c l1 l2 st1 st2 stk lf,
+  | ME_r_pure : forall fc c l1 st1 st2 stk lf,
+      ceval' fc c l1 (com_to_label_pure c) st1 st2 ->
+      middle_ceval' fc lf ((c, Some l1, st1) :: stk) ((c, None, st2) :: stk)
+  | ME_r_single : forall fc c l1 l2 st1 st2 stk lf,
+      single_point l2 ->
       ceval' fc c l1 l2 st1 st2 ->
-      middle_ceval' fc lf ((c, l1, st1) :: stk) ((c, l2, st2) :: stk)
+      middle_ceval' fc lf ((c, Some l1, st1) :: stk) ((c, Some l2, st2) :: stk)
   | ME_re : forall fc c1 c2 l1 loc1 loc2 glb stk lf f,
       In f lf ->
       c2 = snd (fc f) ->
       single_point l1 ->
-      middle_ceval' fc lf ((c1, l1, (loc1, glb)) :: stk)
-        ((c2, com_to_label_pure c2, (loc2, glb)) :: (c1, l1, (loc1, glb)) :: stk)
+      middle_ceval' fc lf ((c1, Some l1, (loc1, glb)) :: stk)
+        ((c2, Some (com_to_label_pure c2), (loc2, glb)) :: (c1, Some l1, (loc1, glb)) :: stk)
   | ME_ex : forall fc c1 c2 l2 loc1 loc2 glb1 glb2 stk lf,
       single_point l2 ->
       middle_ceval' fc lf
-        ((c1, (com_to_label_pure c1), (loc1, glb1)) :: (c2, l2, (loc2, glb2)) :: stk)
-        ((c2, l2, (loc2, glb1)) :: stk).
+        ((c1, None, (loc1, glb1)) :: (c2, Some l2, (loc2, glb2)) :: stk)
+        ((c2, Some l2, (loc2, glb1)) :: stk).
 
 Print clos_trans.
 Search clos_trans_1n.
@@ -237,9 +311,18 @@ Inductive clos_trans (A : Type) (R : relation A) (x : A) : A -> Prop :=
 Definition multi_ceval' (fc : func_context) (lf : public_funcs) : restk -> restk -> Prop :=
   clos_trans restk (middle_ceval' fc lf).
 
-Lemma middle_ceval'_pure : forall fc c l1 l2 st1 st2 lf,
-  middle_ceval' fc lf ((c, l1, st1) :: nil) ((c, l2, st2) :: nil) ->
+Lemma middle_ceval'_some : forall fc c l1 l2 st1 st2 lf,
+  middle_ceval' fc lf ((c, Some l1, st1) :: nil) ((c, Some l2, st2) :: nil) ->
   ceval' fc c l1 l2 st1 st2.
+Proof.
+  intros.
+  inversion H; subst.
+  exact H9.
+Qed.
+
+Lemma middle_ceval'_none : forall fc c l1 st1 st2 lf,
+  middle_ceval' fc lf ((c, Some l1, st1) :: nil) ((c, None, st2) :: nil) ->
+  ceval' fc c l1 (com_to_label_pure c) st1 st2.
 Proof.
   intros.
   inversion H; subst.
@@ -257,29 +340,560 @@ Definition ceval'_derive_multi_ceval : Prop :=
   forall fc lf c st1 st2,
   ceval fc lf c st1 st2 ->
   multi_ceval' fc lf
-    ((c, com_to_label_pure c, st1) :: nil)
-    ((c, com_to_label_pure c, st2) :: nil).
+    ((c, Some (com_to_label_pure c), st1) :: nil)
+    ((c, None, st2) :: nil).
 
 Definition arbitrary_eval_derive_multi_ceval : Prop :=
   forall fc lf loc glb1 glb2 lb c stk,
   single_point lb ->
   arbitrary_eval fc lf loc glb1 glb2 ->
   multi_ceval' fc lf
-    ((c, lb, (loc, glb1)) :: stk)
-    ((c, lb, (loc, glb2)) :: stk).
+    ((c, Some lb, (loc, glb1)) :: stk)
+    ((c, Some lb, (loc, glb2)) :: stk).
 
-
-Lemma com_extension_head :
-  forall fc lf c2 l2 st4 st3 c1,
-  clos_trans restk (middle_ceval' fc lf)
-      ((c2, l2, st4) :: nil)
-      ((c2, com_to_label_pure c2, st3) :: nil) ->
-  clos_trans restk (middle_ceval' fc lf)
-      ((CSeq c1 c2, LSeq (com_to_label_pure c1) l2, st4) :: nil)
-      ((CSeq c1 c2, LSeq (com_to_label_pure c1) (com_to_label_pure c2), st3) :: nil).
+(** Seq Head *)
+Lemma middle_ceval'_seq_head1:
+  forall l1 fc lf c2 st1 st2 stk c1,
+  single_point l1 ->
+  middle_ceval' fc lf
+    ((c2, Some l1, st1) :: stk)
+    ((c2, None, st2) :: stk) ->
+  middle_ceval' fc lf
+    ((CSeq c1 c2, Some (LSeq (com_to_label_pure c1) l1), st1) :: stk)
+    ((CSeq c1 c2, None, st2) :: stk).
 Proof.
   intros.
-Admitted.
+  inversion H0; subst.
+  eapply E'_Seq2 in H4.
+  - apply ME_r_pure.
+    exact H4.
+  - exact H.
+  - apply com_to_label_pure_valid.
+Qed.
+
+Lemma increase_one_side {A : Type}:
+  forall (a : A) l l',
+  ~(l' ++ a :: l = l).
+Proof.
+  unfold not.
+  intros.
+  assert (length (l' ++ a :: l) = length l).
+  rewrite H. auto.
+  rewrite app_length in H0.
+  simpl in H0.
+  omega.
+Qed.
+
+Lemma increase_one_side1 {A : Type}:
+  forall (a b : A) l l',
+  a <> b ->
+  ~(l' ++ a :: l = b :: l).
+Proof.
+  unfold not.
+  intros.
+  destruct l'.
+  - inversion H0.
+    auto.
+  - assert (length ((a0 :: l') ++ a :: l) = length (b :: l)).
+    rewrite H0. auto.
+    rewrite app_length in H1.
+    simpl in H1.
+    omega.
+Qed.
+
+Lemma middle_ceval'_seq_head2:
+  forall l1 l2 fc lf c2 st1 st2 stk c1,
+  single_point l1 ->
+  middle_ceval' fc lf
+    ((c2, Some l1, st1) :: stk)
+    ((c2, Some l2, st2) :: stk) ->
+  middle_ceval' fc lf
+    ((CSeq c1 c2, Some (LSeq (com_to_label_pure c1) l1), st1) :: stk)
+    ((CSeq c1 c2, Some (LSeq (com_to_label_pure c1) l2), st2) :: stk).
+Proof.
+  intros.
+  inversion H0; subst.
+  eapply E'_Seq2 in H10.
+  - apply ME_r_single.
+    apply SP_Seq2.
+    apply com_to_label_pure_is_pure.
+    exact H5.
+    exact H10.
+  - exact H.
+  - right.
+    exact H5.
+  - pose proof increase_one_side (snd (fc f), Some l1, (loc1, glb)) stk nil.
+    simpl in H1.
+    congruence.
+Qed.
+
+Lemma middle_ceval'_seq_head_some:
+  forall fc lf c1 c2 l1 l2 st1 st2 stk1 stk2,
+  single_point l1 ->
+  middle_ceval' fc lf
+    (stk1 ++ (c2, Some l1, st1) :: nil)
+    (stk2 ++ (c2, Some l2, st2) :: nil) ->
+  middle_ceval' fc lf
+    (stk1 ++ (CSeq c1 c2, Some (LSeq (com_to_label_pure c1) l1), st1) :: nil)
+    (stk2 ++ (CSeq c1 c2, Some (LSeq (com_to_label_pure c1) l2), st2) :: nil).
+Proof.
+  intros.
+  destruct stk1, stk2; simpl in *.
+  - inversion H0; subst.
+    apply middle_ceval'_seq_head2; assumption.
+  - inversion H0; subst.
+    + assert (@length (com * option label * state) nil = length (stk2 ++ (c2, Some l2, st2) :: nil)).
+      rewrite H9 at 1. auto.
+      rewrite app_length in H1.
+      simpl in H1. omega.
+    + assert (@length (com * option label * state) nil = length (stk2 ++ (c2, Some l2, st2) :: nil)).
+      rewrite H9 at 1. auto.
+      rewrite app_length in H1.
+      simpl in H1. omega.
+    + destruct stk2; simpl in *.
+      2:{
+        assert (length ((c2, Some l1, (loc1, glb)) :: nil) = length (p :: stk2 ++ (c2, Some l2, st2) :: nil)).
+        rewrite <- H9. auto.
+        simpl in H1.
+        rewrite app_length in H1.
+        simpl in H1.
+        omega.
+      }
+      rewrite <- app_nil_l in H9 at 1.
+      rewrite <- app_nil_l in H9.
+      apply app_inj_tail in H9.
+      destruct H9 as [_ ?].
+      inversion H1; subst. clear H1.
+      eapply ME_re.
+      * exact H6.
+      * auto.
+      * apply SP_Seq2.
+        apply com_to_label_pure_is_pure.
+        exact H11.
+  - inversion H0; subst.
+    + assert (length (stk1 ++ (c2, Some l1, st1) :: nil) = @length (com * option label * state) nil).
+      rewrite H9. auto.
+      rewrite app_length in H1.
+      simpl in H1.
+      omega.
+    + destruct stk1; simpl in *.
+      2:{
+        assert (length ((c2, Some l2, (loc2, glb2)) :: nil) = length (p :: stk1 ++ (c2, Some l1, st1) :: nil)).
+        rewrite <- H5. auto.
+        simpl in H1.
+        rewrite app_length in H1.
+        simpl in H1.
+        omega.
+      }
+      rewrite <- app_nil_l in H5 at 1.
+      rewrite <- app_nil_l in H5.
+      apply app_inj_tail in H5.
+      destruct H5 as [_ ?].
+      inversion H1; subst; clear H1.
+      eapply ME_ex.
+      apply SP_Seq2.
+      apply com_to_label_pure_is_pure.
+      exact H4.
+  - inversion H0; subst.
+    + apply app_inj_tail in H7.
+      destruct H7.
+      inversion H2; subst.
+      apply ME_r_pure.
+      exact H4.
+    + apply app_inj_tail in H7.
+      destruct H7.
+      inversion H2; subst.
+      apply ME_r_single.
+      exact H6.
+      exact H8.
+    + rewrite app_comm_cons in H6.
+      apply app_inj_tail in H6.
+      destruct H6.
+      inversion H2; subst; clear H2.
+      eapply ME_re.
+      * exact H7.
+      * auto.
+      * exact H9.
+    + rewrite app_comm_cons in H5.
+      apply app_inj_tail in H5.
+      destruct H5.
+      inversion H2; subst; clear H2.
+      apply ME_ex.
+      exact H4.
+Qed.
+
+Lemma middle_ceval'_seq_head_none:
+  forall fc lf c1 c2 l1 st1 st2 stk1 stk2,
+  single_point l1 ->
+  middle_ceval' fc lf
+    (stk1 ++ (c2, Some l1, st1) :: nil)
+    (stk2 ++ (c2, None, st2) :: nil) ->
+  middle_ceval' fc lf
+    (stk1 ++ (CSeq c1 c2, Some (LSeq (com_to_label_pure c1) l1), st1) :: nil)
+    (stk2 ++ (CSeq c1 c2, None, st2) :: nil).
+Proof.
+  intros.
+  destruct stk1, stk2; simpl in *.
+  - inversion H0; subst.
+    apply middle_ceval'_seq_head1; assumption.
+  - inversion H0; subst.
+    + assert (@length (com * option label * state) nil = length (stk2 ++ (c2, None, st2) :: nil)).
+      rewrite H9 at 1. auto.
+      rewrite app_length in H1.
+      simpl in H1. omega.
+    + assert (@length (com * option label * state) nil = length (stk2 ++ (c2, None, st2) :: nil)).
+      rewrite H9 at 1. auto.
+      rewrite app_length in H1.
+      simpl in H1. omega.
+    + destruct stk2; simpl in *.
+      2:{
+        assert (length ((c2, Some l1, (loc1, glb)) :: nil) = length (p :: stk2 ++ (c2, None, st2) :: nil)).
+        rewrite <- H9. auto.
+        simpl in H1.
+        rewrite app_length in H1.
+        simpl in H1.
+        omega.
+      }
+      rewrite <- app_nil_l in H9 at 1.
+      rewrite <- app_nil_l in H9.
+      apply app_inj_tail in H9.
+      destruct H9 as [_ ?].
+      inversion H1.
+  - inversion H0; subst.
+    + assert (length (stk1 ++ (c2, Some l1, st1) :: nil) = @length (com * option label * state) nil).
+      rewrite H8. auto.
+      rewrite app_length in H1.
+      simpl in H1.
+      omega.
+  - inversion H0; subst.
+    + apply app_inj_tail in H7.
+      destruct H7.
+      inversion H2.
+    + apply app_inj_tail in H7.
+      destruct H7.
+      inversion H2.
+    + rewrite app_comm_cons in H6.
+      apply app_inj_tail in H6.
+      destruct H6.
+      inversion H2.
+    + rewrite app_comm_cons in H5.
+      apply app_inj_tail in H5.
+      destruct H5.
+      inversion H2.
+Qed.
+
+Lemma cons_insert_nil {A : Type} :
+  forall (a : A) l,
+  a :: l = a :: nil ++ l.
+Proof.
+  intros.
+  auto.
+Qed.
+
+Lemma multi_ceval'_seq_head:
+  forall l2 fc lf c2 st4 st3 c1,
+  single_point l2 ->
+  clos_trans restk (middle_ceval' fc lf)
+      ((c2, Some l2, st4) :: nil)
+      ((c2, None, st3) :: nil) ->
+  clos_trans restk (middle_ceval' fc lf)
+      ((CSeq c1 c2, Some (LSeq (com_to_label_pure c1) l2), st4) :: nil)
+      ((CSeq c1 c2, None, st3) :: nil).
+Proof.
+  intros.
+  set (stk := @nil (com * option label * state)).
+  unfold stk.
+  change ((c2, Some l2, st4) :: nil) with (stk ++ ((c2, Some l2, st4) :: nil)) in H0.
+  change ((CSeq c1 c2, Some (LSeq (com_to_label_pure c1) l2), st4) :: nil) with (stk ++ ((CSeq c1 c2, Some (LSeq (com_to_label_pure c1) l2), st4) :: nil)).
+  clearbody stk.
+  remember (stk ++ ((c2, Some l2, st4) :: nil)) as l.
+  remember ((c2, None, st3) :: nil) as l'.
+  apply Operators_Properties.clos_trans_t1n in H0.
+  revert Heql.
+  revert stk st4.
+  revert c1.
+  generalize dependent l2.
+  induction H0; intros; subst.
+  - rewrite <- app_nil_l in H.
+    eapply middle_ceval'_seq_head_none, t_step in H.
+    simpl in H. exact H. exact H0.
+  - inversion H; subst.
+    + specialize (IHclos_trans_1n (eq_refl _) l2 H1).
+      destruct stk.
+      * destruct stk0.
+        inversion H0; inversion H3.
+        assert (length ((c, Some l1, st1) :: p :: stk0) = length (nil ++ (c2, Some l2, st4) :: nil)).
+        rewrite H2. auto.
+        simpl in H3. omega.
+      * simpl in H2.
+        inversion H2; subst; clear H2.
+        simpl in *.
+        pose proof IHclos_trans_1n c1 ((c, None, st2) :: stk) st4.
+        specialize (H2 (eq_refl _)).
+        repeat rewrite app_comm_cons in H.
+        eapply middle_ceval'_seq_head_some, t_step in H.
+        simpl in *.
+        eapply t_trans.
+        exact H. exact H2. exact H1.
+    + destruct stk.
+      * destruct stk0.
+        2:{
+          pose proof (eq_refl (length ((c, Some l1, st1) :: p :: stk0))).
+          rewrite H2 in H4 at 1.
+          simpl in H4. omega.
+        }
+        simpl in *.
+        inversion H2; subst; clear H2.
+        pose proof (IHclos_trans_1n (eq_refl _) l0 H3 c1 nil st2 (eq_refl _)).
+        simpl in *.
+        eapply middle_ceval'_seq_head2, t_step in H.
+        eapply t_trans.
+        exact H. exact H2. exact H1.
+      * simpl in H2.
+        inversion H2; subst; clear H2.
+        pose proof (IHclos_trans_1n (eq_refl _) l2 H1 c1 ((c, Some l0, st2) :: stk) st4 (eq_refl _)).
+        rewrite app_comm_cons in H.
+        eapply middle_ceval'_seq_head_some, t_step in H.
+        eapply t_trans.
+        exact H. exact H2. exact H1.
+    + destruct stk.
+      * destruct stk0.
+        2:{
+          pose proof (eq_refl (length ((c0, Some l1, (loc1, glb)) :: p :: stk0))).
+          rewrite H2 in H4 at 1.
+          simpl in H4. omega.
+        }
+        simpl in *.
+        inversion H2; subst; clear H2.
+        pose proof IHclos_trans_1n (eq_refl _) l2 H1 c1 ((snd (fc f), Some (com_to_label_pure (snd (fc f))), (loc2, glb)) :: nil) (loc1, glb) (eq_refl _).
+        assert ((c2, Some l2, (loc1, glb)) :: nil = nil ++ (c2, Some l2, (loc1, glb)) :: nil). auto.
+        pose proof middle_ceval'_seq_head_some fc lf c1 c2 l2 l2 (loc1, glb) (loc1, glb) nil. simpl in H5.
+        assert ((snd (fc f), Some (com_to_label_pure (snd (fc f))), (loc2, glb)) :: (c2, Some l2, (loc1, glb)) :: nil = ((snd (fc f), Some (com_to_label_pure (snd (fc f))), (loc2, glb)) :: nil) ++ (c2, Some l2, (loc1, glb)) :: nil). auto.
+        rewrite H6 in H; clear H6.
+        eapply H5, t_step in H.
+        eapply t_trans.
+        exact H. exact H2. exact H1.
+      * simpl in H2; inversion H2; subst; clear H2.
+        pose proof IHclos_trans_1n (eq_refl _) l2 H1 c1 ((snd (fc f), Some (com_to_label_pure (snd (fc f))), (loc2, glb)) :: (c0, Some l1, (loc1, glb)) :: stk) st4 (eq_refl _).
+        rewrite app_comm_cons in H. rewrite app_comm_cons in H.
+        eapply middle_ceval'_seq_head_some, t_step in H.
+        eapply t_trans.
+        exact H. exact H2. exact H1.
+  + destruct stk.
+    simpl in H2.
+    pose proof eq_refl (length ((c2, Some l2, st4) :: nil)).
+    rewrite <- H2 in H3 at 1.
+    simpl in H3. omega.
+    simpl in H2.
+    destruct stk.
+    * simpl in H2.
+      inversion H2; subst; clear H2.
+      pose proof IHclos_trans_1n (eq_refl _) l2 H1 c1 nil (loc2, glb1) (eq_refl _).
+      simpl in H2.
+      rewrite <- app_nil_l in H.
+      eapply middle_ceval'_seq_head_some, t_step in H.
+      eapply t_trans.
+      exact H. exact H2. exact H1.
+    * simpl in *.
+      inversion H2; subst; clear H2.
+      pose proof IHclos_trans_1n (eq_refl _) l2 H1 c1 ((c3, Some l0, (loc2, glb1)) :: stk) st4 (eq_refl _).
+      repeat rewrite app_comm_cons in H.
+      eapply middle_ceval'_seq_head_some, t_step in H.
+      eapply t_trans.
+      exact H. exact H2. exact H1.
+Qed.
+(** Seq Head *)
+
+(** Seq Tail *)
+Lemma middle_ceval'_seq_tail:
+  forall fc lf c1 st1 stk1 stk2 l0 l1 st0 c2,
+  single_point l1 ->
+  middle_ceval' fc lf
+    (stk1 ++ (c1, Some l0, st1) :: nil)
+    (stk2 ++ (c1, Some l1, st0) :: nil) ->
+  middle_ceval' fc lf
+    (stk1 ++ (CSeq c1 c2, Some (LSeq l0 (com_to_label_pure c2)), st1) :: nil)
+    (stk2 ++ (CSeq c1 c2, Some (LSeq l1 (com_to_label_pure c2)), st0) :: nil).
+Proof.
+  intros.
+  destruct stk1, stk2; simpl in *.
+  - inversion H0; subst.
+    eapply E'_Seq1 in H10.
+    apply ME_r_single.
+    apply SP_Seq1.
+    exact H.
+    apply com_to_label_pure_is_pure.
+    exact H10.
+    apply ceval'_valid_label in H10.
+    tauto.
+    exact H.
+  - inversion H0; subst.
+    + pose proof eq_refl (@length (com * option label * state) nil).
+      rewrite H9 in H1 at 1.
+      rewrite app_length in H1.
+      simpl in H1. omega.
+    + pose proof eq_refl (@length (com * option label * state) nil).
+      rewrite H9 in H1 at 1.
+      rewrite app_length in H1.
+      simpl in H1. omega.
+    + destruct stk2; simpl in *.
+      * inversion H9; subst; clear H9.
+        eapply ME_re.
+        exact H6.
+        apply eq_refl.
+        apply SP_Seq1.
+        exact H11.
+        apply com_to_label_pure_is_pure.
+      * pose proof eq_refl (length (p :: stk2 ++ (c1, Some l1, st0) :: nil)).
+        rewrite <- H9 in H1 at 1.
+        simpl in H1.
+        rewrite app_length in H1.
+        simpl in H1. omega.
+  - inversion H0; subst.
+    + pose proof eq_refl (@length (com * option label * state) nil).
+      rewrite <- H9 in H1 at 1.
+      rewrite app_length in H1.
+      simpl in H1. omega.
+    + destruct stk1; simpl in *.
+      * inversion H5; subst.
+        apply ME_ex.
+        apply SP_Seq1.
+        exact H4.
+        apply com_to_label_pure_is_pure.
+      * pose proof eq_refl (length ((c1, Some l1, (loc2, glb2)) :: nil)).
+        rewrite H5 in H1 at 1.
+        simpl in H1.
+        rewrite app_length in H1.
+        simpl in H1. omega.
+  - inversion H0; subst.
+    + apply app_inj_tail in H7;
+      destruct H7; inversion H2; subst; clear H2.
+      eapply ME_r_pure in H4.
+      apply H4.
+    + apply app_inj_tail in H7;
+      destruct H7; inversion H2; subst; clear H2.
+      eapply ME_r_single in H8.
+      apply H8.
+      exact H6.
+    + destruct stk2; simpl in *.
+      * pose proof eq_refl (length ((c1, Some l1, st0) :: nil)).
+        rewrite <- H6 in H1 at 1.
+        simpl in H1.
+        rewrite app_length in H1.
+        simpl in H1. omega.
+      * inversion H6; subst; clear H6.
+        apply app_inj_tail in H3 as [? ?].
+        inversion H2; subst; clear H2.
+        eapply ME_re.
+        exact H7.
+        auto.
+        exact H9.
+    + destruct stk1; simpl in *.
+      * pose proof eq_refl (length ((c1, Some l0, st1) :: nil)).
+        rewrite <- H5 in H1 at 1.
+        simpl in H1.
+        rewrite app_length in H1.
+        simpl in H1. omega.
+      * inversion H5; subst; clear H5.
+        apply app_inj_tail in H3 as [? ?].
+        inversion H2; subst; clear H2.
+        eapply ME_ex.
+        exact H4.
+Qed.
+
+Lemma multi_ceval'_seq_tail:
+  forall fc lf c1 c2 l1 st1 st0,
+  single_point l1 ->
+  clos_trans restk (middle_ceval' fc lf)
+    ((c1, Some (com_to_label_pure c1), st1) :: nil)
+    ((c1, Some l1, st0) :: nil) ->
+  clos_trans restk (middle_ceval' fc lf)
+    ((CSeq c1 c2, Some (LSeq (com_to_label_pure c1) (com_to_label_pure c2)), st1) :: nil)
+    ((CSeq c1 c2, Some (LSeq l1 (com_to_label_pure c2)), st0) :: nil).
+Proof.
+  intros.
+  set (stk := @nil (com * option label * state)).
+  unfold stk.
+  change ((c1, Some l1, st0) :: nil) with (stk ++ ((c1, Some l1, st0) :: nil)) in H0.
+  change ((CSeq c1 c2, Some (LSeq l1 (com_to_label_pure c2)), st0) :: nil) with (stk ++ ((CSeq c1 c2, Some (LSeq l1 (com_to_label_pure c2)), st0) :: nil)).
+  clearbody stk.
+  remember (stk ++ ((c1, Some l1, st0) :: nil)) as l.
+  remember ((c1, Some (com_to_label_pure c1), st1) :: nil) as l'.
+  apply Operators_Properties.clos_trans_tn1 in H0.
+  revert Heql.
+  revert stk st0.
+  revert c2.
+  generalize dependent l1.
+  induction H0; intros; subst.
+  - change ((c1, Some (com_to_label_pure c1), st1) :: nil) with (nil ++ (c1, Some (com_to_label_pure c1), st1) :: nil) in H.
+    eapply middle_ceval'_seq_tail, t_step in H.
+    simpl in H. exact H. exact H0.
+  - inversion H; subst.
+    + destruct stk; simpl in *; inversion H2; subst; clear H2.
+      pose proof IHclos_trans_n1 l1 H1 c2 ((c, Some l0, st2) :: stk) st0 (eq_refl _).
+      repeat rewrite app_comm_cons in H.
+      eapply middle_ceval'_seq_tail, t_step in H.
+      eapply t_trans.
+      exact H2. exact H. exact H1.
+    + destruct stk; simpl in *.
+      * inversion H2; subst; clear H2.
+        change ((c1, Some l0, st2) :: nil) with (nil ++ (c1, Some l0, st2) :: nil) in H.
+        change ((c1, Some l1, st0) :: nil) with (nil ++ (c1, Some l1, st0) :: nil) in H.
+        eapply middle_ceval'_seq_tail, t_step in H.
+        epose proof IHclos_trans_n1 l0 _ c2 nil st2 (eq_refl _).
+        simpl in *.
+        eapply t_trans.
+        exact H2. exact H. exact H3.
+      * inversion H2; subst; clear H2.
+        pose proof IHclos_trans_n1 l1 H1 c2 ((c, Some l0, st2) :: stk) st0 (eq_refl _).
+        repeat rewrite app_comm_cons in H.
+        eapply middle_ceval'_seq_tail, t_step in H.
+        simpl in *.
+        eapply t_trans.
+        exact H2. exact H. exact H1.
+    + destruct stk; simpl in *.
+      * pose proof eq_refl (length ((c1, Some l1, st0) :: nil)).
+        rewrite <- H2 in H4 at 1.
+        simpl in H4. omega.
+      * inversion H2; subst.
+        destruct stk; simpl in *.
+        {
+          inversion H6; subst.
+          clear H2 H6.
+          pose proof IHclos_trans_n1 l1 H1 c2 nil (loc1, glb) (eq_refl _).
+          rewrite <- (@app_nil_l (_ * _ * _)) in H at 1.
+          pose proof cons_insert_nil (snd (fc f), Some (com_to_label_pure (snd (fc f))), (loc2, glb)).
+          rewrite H4, app_comm_cons in H; clear H4.
+          eapply middle_ceval'_seq_tail, t_step in H.
+          eapply t_trans.
+          exact H2. exact H. exact H1.
+        }
+        {
+          inversion H6; subst; clear H2 H6.
+          pose proof IHclos_trans_n1 l1 H1 c2 ((c0, Some l0, (loc1, glb)) :: stk) st0 (eq_refl _).
+          repeat rewrite app_comm_cons in H.
+          eapply middle_ceval'_seq_tail, t_step in H.
+          eapply t_trans.
+          exact H2. exact H. exact H1.
+        }
+    + destruct stk; simpl in *.
+      * inversion H2; subst; clear H2.
+        pose proof IHclos_trans_n1 l1 H1 c2 ((c0, None, (loc1, glb1)) :: nil) (loc2, glb2) (eq_refl _).
+        rewrite <- app_nil_l in H.
+        rewrite cons_insert_nil, app_comm_cons in H.
+        eapply middle_ceval'_seq_tail, t_step in H.
+        eapply t_trans.
+        exact H2. exact H. exact H1.
+      * inversion H2; subst; clear H2.
+        pose proof IHclos_trans_n1 l1 H1 c2 ((c0, None, (loc1, glb1)) :: (c3, Some l2, (loc2, glb2)) :: stk) st0 (eq_refl _).
+        repeat rewrite app_comm_cons in H.
+        eapply middle_ceval'_seq_tail, t_step in H.
+        eapply t_trans.
+        exact H2. exact H. exact H1.
+Unshelve.
+  inversion H0; inversion H2; assumption.
+Qed.
+(** Seq Tail *)
 
 Theorem ceval'_derive_multi_ceval_correct : ceval'_derive_multi_ceval.
 Proof.
@@ -287,60 +901,97 @@ Proof.
   intros.
   induction H.
   - simpl.
-    apply t_step, ME_r.
-    apply E'_Skip.
+    apply t_step, ME_r_pure.
+    simpl. apply E'_Skip.
   - simpl.
-    apply t_step, ME_r.
-    apply E'_Ass, H.
+    apply t_step, ME_r_pure.
+    simpl. apply E'_Ass, H.
   - simpl.
     apply Operators_Properties.clos_trans_tn1 in IHceval1.
     apply Operators_Properties.clos_trans_t1n in IHceval2.
     inversion IHceval1; subst; inversion IHceval2; subst.
-    + apply middle_ceval'_pure in H1.
-      apply middle_ceval'_pure in H2.
+    + apply middle_ceval'_none in H1.
+      apply middle_ceval'_none in H2.
       epose proof E'_Seq _ _ _ _ _ _ _ _ _ _ _ _ _ _ H1 H2.
-      apply t_step, ME_r.
+      apply t_step, ME_r_pure.
       exact H3.
-    + apply middle_ceval'_pure in H1.
+    + apply middle_ceval'_none in H1.
       inversion H2; subst.
-      * epose proof E'_Seq _ _ _ _ _ _ _ _ _ _ _ _ _ _ H1 H11.
-        Search clos_trans_1n clos_trans.
+      * inversion H3; inversion H4.
+      * assert (valid_label l2) as Htmp. right. assumption.
+      pose proof E'_Seq fc c1 c2 (com_to_label_pure c1) (com_to_label_pure c1) (com_to_label_pure c2) l2 _ _ _ (com_to_label_pure_valid _) (com_to_label_pure_is_pure _) (com_to_label_pure_is_pure _) Htmp H1 H12.
+        clear Htmp.
         apply Operators_Properties.clos_t1n_trans in H3.
-        eapply com_extension_head in H3.
+        eapply ME_r_single in H4.
+        2:{
+          apply SP_Seq2, H11.
+          apply com_to_label_pure_is_pure.
+        }
         apply Operators_Properties.clos_t1n_trans.
         eapply t1n_trans.
+        apply H4.
+        clear H4.
+        eapply multi_ceval'_seq_head in H3.
+        apply Operators_Properties.clos_trans_t1n.
+        exact H3.
+        exact H11.
+      * pose proof com_to_label_pure_no_point c2.
+        tauto.
+    + apply middle_ceval'_none in H3.
+      inversion H1; subst.
+      * pose proof ceval'_valid_label _ _ _ _ _ _ H8 as [Htmp _].
+        pose proof E'_Seq _ _ _ _ _ _ _ _ _ _ Htmp (com_to_label_pure_is_pure _) (com_to_label_pure_is_pure _) (com_to_label_pure_valid _) H8 H3.
+        clear Htmp.
+        apply Operators_Properties.clos_tn1_trans in H2.
+        eapply ME_r_pure, t_step in H4.
+        eapply multi_ceval'_seq_tail in H2.
+        eapply t_trans.
+        apply H2. apply H4.
+        apply Operators_Properties.clos_trans_tn1 in H2.
+        inversion H2; inversion H5; assumption.
+    + inversion H1; subst; inversion H3; subst.
+      * inversion H4; inversion H5.
+      * pose proof ceval'_valid_label _ _ _ _ _ _ H9 as [Htmp1 _].
+        pose proof ceval'_valid_label _ _ _ _ _ _ H14 as [_ Htmp2].
+        pose proof E'_Seq _ _ _ _ _ _ _ _ _ _ Htmp1 (com_to_label_pure_is_pure _) (com_to_label_pure_is_pure _) Htmp2 H9 H14.
+        apply Operators_Properties.clos_tn1_trans in H2.
+        apply Operators_Properties.clos_t1n_trans in H4.
+        eapply multi_ceval'_seq_tail in H2.
+        eapply multi_ceval'_seq_head in H4.
+        eapply ME_r_single, t_step in H5.
         {
-          apply ME_r.
+          eapply t_trans.
+          apply H2.
+          eapply t_trans.
+          apply H5.
           apply H4.
         }
         {
-          apply Operators_Properties.clos_trans_t1n.
-          exact H3.
+          apply SP_Seq2.
+          apply com_to_label_pure_is_pure.
+          assumption.
         }
+        assumption.
+        inversion H2.
+        {
+          inversion H6; subst.
+          assumption.
+        }
+        apply Operators_Properties.clos_trans_tn1 in H2.
+        inversion H2; inversion H10; assumption.
       * pose proof com_to_label_pure_no_point c2.
         tauto.
-    + apply middle_ceval'_pure in H3.
-      inversion H1; subst.
-      * epose proof E'_Seq _ _ _ _ _ _ _ _ _ _ _ _ _ _ H8 H3.
-        admit.
-      * pose proof com_to_label_pure_no_point c1.
-        tauto.
-    + inversion H1; subst; inversion H3; subst.
-      * epose proof E'_Seq _ _ _ _ _ _ _ _ _ _ _ _ _ _ H9 H13.
-        admit.
-      * pose proof com_to_label_pure_no_point c2.
-        tauto.
-      * pose proof com_to_label_pure_no_point c1.
-        tauto.
-      * pose proof com_to_label_pure_no_point c1.
-        tauto.
-    apply t_step, ME_r.
-    eapply E'_Seq.
-    apply com_to_label_pure_valid.
-    apply com_to_label_pure_is_pure.
-    apply com_to_label_pure_is_pure.
-    apply com_to_label_pure_valid.
-    
+  - admit.
+  - admit.
+  - admit.
+  - admit.
+  - admit.
+Unshelve.
+  left. apply com_to_label_pure_is_pure.
+  apply com_to_label_pure_is_pure.
+  apply com_to_label_pure_is_pure.
+  left. apply com_to_label_pure_is_pure.
+Admitted.
 (*   remember (snd (fc f)) as c.
   revert f Heqc.
   induction H; intros.
